Lem.dfy
@@ -4,8 +4,8 @@ module Lem {
   import opened Type
   import opened Property
 
-  lemma bst_meaning(t:Rb_tree)
-    requires t.Node? && bst_property(t)
+  lemma bstMeaning(t:Rb_tree)
+    requires t.Node? && bstProperty(t)
     ensures !t.left.Node? || t.left.key < t.key
     ensures !t.right.Node? || t.right.key > t.key
   {
@@ -17,26 +17,26 @@ module Lem {
     assert forall x :: x in contain(t.right) ==> x > t.key;
     // assert t.right.key > t.key;
   }
-  lemma bst_transitivity_right(t:Rb_tree)
-    requires t.Node? &&t.left.Node? && bst_property(t)
+  lemma bstTransitivityRight(t:Rb_tree)
+    requires t.Node? &&t.left.Node? && bstProperty(t)
     ensures forall x :: x in contain (t.left.right)==> x < t.key
 
   {
-    assert bst_property(t);
-    assert bst_property(t.left);
-    assert bst_property(t.right);
+    assert bstProperty(t);
+    assert bstProperty(t.left);
+    assert bstProperty(t.right);
     assert forall x :: x in contain(t.left.right) ==> x in contain(t.left);
 
   }
 
-  lemma bst_transitivity_left(t:Rb_tree)
-    requires t.Node? && t.right.Node? && bst_property(t)
+  lemma bstTransitivityLeft(t:Rb_tree)
+    requires t.Node? && t.right.Node? && bstProperty(t)
     ensures forall x :: x in contain (t.right.left)==> x > t.key
 
   {
-    assert bst_property(t);
-    assert bst_property(t.right);
-    assert bst_property(t.left);
+    assert bstProperty(t);
+    assert bstProperty(t.right);
+    assert bstProperty(t.left);
     assert forall x :: x in contain(t.right.left) ==> x in contain(t.right);
   }
 
@@ -51,27 +51,8 @@ module Lem {
   {
   }
 
-  // lemma {:axiom} DLL_Contradicts_WeakLLRB_Child(h_node: Rb_tree)
-  //   requires h_node.Node? && h_node.left.Node?
-  //   requires weakLLRB(h_node.left) // If h.left was l_rec directly
-  //   requires double_left_red_link(h_node)
-  //   ensures false
-  // {
-  //   var N := h_node.left; // N is l_rec
-  //   assert N.color == Red; // From double_left_red_link(h_node)
-  //   assert N.left.Node? && N.left.color == Red; // From double_left_red_link(h_node)
-  //   // weakLLRB(N) implies goodColor(N).
-  //   // goodColor(N) when N is Red implies N.left is Black.
-  //   // This establishes the contradiction. Unfold definitions if necessary.
-  //   if N.Node? && N.color == Red && weakLLRB(N) { // Trigger unfolding of weakLLRB
-  //     assert N.Node? && N.color == Red && strongLLRB(N.left);
-  //     assume nodeColor(N.left) == Black; // By goodColor part of weakLLRB(N)
-  //   }
-  //   // Now we have N.left.color == Red and N.left.color == Black
-  //   assert N.left.color == Black && N.left.color == Red; // Should lead to false
-  // }
 
-  lemma black_promote(t: Rb_tree)
+  lemma blackPromote(t: Rb_tree)
     ensures (isBlack(t) && weakLLRB(t)) ==> strongLLRB(t)
   {
   }
@@ -82,17 +63,22 @@ module Lem {
     requires l_child.Null? || (isBlack(l_child) && strongLLRB(l_child))
     requires r_child.Null? || (isBlack(r_child) && strongLLRB(r_child))
     requires BlackHeight(l_child) == BlackHeight(r_child)
-    requires bst_property(n)
+    requires bstProperty(n)
     ensures strongLLRB(n)
   {
   }
 
-  lemma color_dont_change_color(t_orig: Rb_tree, new_color: Color)
+  lemma color_dont_change_bst(t_orig: Rb_tree, new_color: Color)
     requires t_orig.Node?
-    requires bst_property(t_orig)
-    ensures bst_property(Node(new_color, t_orig.key, t_orig.left, t_orig.right))
+    requires bstProperty(t_orig)
+    ensures bstProperty(Node(new_color, t_orig.key, t_orig.left, t_orig.right))
     ensures contain(Node(new_color, t_orig.key, t_orig.left, t_orig.right)) == contain(t_orig)
   {
-    var t_new := Node(new_color, t_orig.key, t_orig.left, t_orig.right);
+  }
+
+  lemma strongRedRightBlack (t: Rb_tree)
+    ensures (strongLLRB(t) && isRed(t)) ==> isBlack(t.right)
+  {
+
   }
 }
