Operations.dfy
@@ -6,8 +6,8 @@ module Operations {
   import opened Property
   import opened Lem
 
-  // This is the pre-condition for rotate_left
-  predicate right_leaning_red_link(t: Rb_tree)
+  // This is the pre-condition for rotateLeft
+  predicate rightLeaningRedLink(t: Rb_tree)
   {
     match t
     case Node(_, _, Null, Node(Red, _, _, _)) => true
@@ -15,14 +15,14 @@ module Operations {
     case _ => false
   }
 
-  method rotate_left(h: Rb_tree) returns (result: Rb_tree)
-    requires right_leaning_red_link(h)
-    requires bst_property(h)
+  method rotateLeft(h: Rb_tree) returns (result: Rb_tree)
+    requires rightLeaningRedLink(h)
+    requires bstProperty(h)
     requires BlackHeight(h.left) == BlackHeight(h.right)
     requires BlackHeight(h.right.left) == BlackHeight(h.right.right)
-    ensures !right_leaning_red_link(result)
-    ensures bst_property(result)
-    ensures equal_content_property(h,result)
+    ensures !rightLeaningRedLink(result)
+    ensures bstProperty(result)
+    ensures equalContentProperty(h,result)
     ensures nodeColor(result) == nodeColor(h)
     ensures BlackHeight(result) ==BlackHeight(h)
     ensures contain(h) == contain(result)
@@ -37,28 +37,32 @@ module Operations {
   {
     var new_h := Node(Red, h.key, h.left, h.right.left);
     result := Node(h.color, h.right.key, new_h, h.right.right);
-    bst_meaning(h);
-    bst_transitivity_left(h);
-    assert bst_property(result.left);
-    assert bst_property(result.right);
+    bstMeaning(h);
+    bstTransitivityLeft(h);
+    assert bstProperty(result.left);
+    assert bstProperty(result.right);
     assert result.left.Node?;
     assert h.right.color == Red;
     return;
   }
 
-  method rotate_right(h: Rb_tree) returns (result: Rb_tree)
-    requires double_left_red_link(h)
+  method rotateRight(h: Rb_tree) returns (result: Rb_tree)
+    requires doubleLeftRedLink(h)
     requires BlackHeight(h.left) == BlackHeight(h.right)
     // this is a must
     requires BlackHeight(h.left.left) == BlackHeight(h.left.right)
-    requires bst_property(h)
-    ensures bst_property(result)
+    requires bstProperty(h)
+    ensures bstProperty(result)
     ensures contain(result) == contain(h)
     ensures BlackHeight(result.left) == BlackHeight(result.right)
     ensures BlackHeight(result) == BlackHeight(h)
     ensures result.color == h.color
     ensures isRed(result.left)
     ensures isRed(result.right)
+    ensures  result.left == h.left.left
+    ensures  result.right.left == h.left.right
+    ensures  result.right.right == h.right
+    ensures  nodeColor(result) == nodeColor(h)
     decreases h
   {
     var new_h := Node(Red, h.key, h.left.right, h.right);
@@ -72,14 +76,14 @@ module Operations {
     assert contain(result.right) == contain(h.left.right) + contain(h.right) + {new_h.key};
     assert forall x :: x in contain(h.left.right) ==> x > result.key;
     assert forall x :: x in contain(h.right) ==> x > new_h.key;
-    assert bst_property(result.left);
-    assert bst_property(h);
-    bst_meaning(h);
+    assert bstProperty(result.left);
+    assert bstProperty(h);
+    bstMeaning(h);
     assert forall x :: x in contain(h.left.right) ==> x > h.left.key;
     assert forall x :: x in contain(h.right) ==> x > h.left.key;
-    assert(bst_property(new_h.left));
-    assert bst_property(new_h.right);
-    bst_transitivity_right(h);
+    assert(bstProperty(new_h.left));
+    assert bstProperty(new_h.right);
+    bstTransitivityRight(h);
     assert forall x :: x in contain(new_h.left) ==> x < new_h.key;
     return;
   }
@@ -89,12 +93,16 @@ module Operations {
     requires h.Node? && h.left.Node? && h.right.Node?
     requires h.left.color == Red && h.right.color == Red
     requires BlackHeight(h.left) == BlackHeight(h.right)
-    requires bst_property(h)
+    requires bstProperty(h)
     requires strongLLRB(h)
     ensures strongLLRB(result)
-    ensures bst_property(result)
-    ensures equal_content_property(result, h)
+    ensures bstProperty(result)
+    ensures equalContentProperty(result, h)
     ensures result.Node? && result.left.Node? && result.right.Node?
+    ensures nodeColor(h) == Black ==> (nodeColor(result) == Red && nodeColor(result.left) == Black
+                                       && nodeColor(result.right) == Black)
+    ensures nodeColor(h) == Red ==> (nodeColor(result) == Black && nodeColor(result.left) == Red
+                                     && nodeColor(result.right) == Red)
     ensures  result.left.left   == h.left.left
     ensures  result.left.right  == h.left.right
     ensures  result.right.left  == h.right.left
@@ -104,14 +112,14 @@ module Operations {
     ensures BlackHeight(result) == BlackHeight(h)
     decreases h
   {
-    var new_left_color := (if h.left.color == Red then Black else Red);
-    var new_left := Node(new_left_color, h.left.key, h.left.left, h.left.right);
-    assert bst_property(h.left);
-    assert bst_property(h.right);
-    var new_right_color := (if h.right.color == Red then Black else Red);
-    var new_right := Node(new_right_color, h.right.key, h.right.left, h.right.right);
-    var result_color := ((if h.color == Red then Black else Red));
-    result := Node(result_color, h.key, new_left, new_right);
+    var new_left_nodeColor := (if h.left.color == Red then Black else Red);
+    var new_left := Node(new_left_nodeColor, h.left.key, h.left.left, h.left.right);
+    assert bstProperty(h.left);
+    assert bstProperty(h.right);
+    var new_right_nodeColor := (if h.right.color == Red then Black else Red);
+    var new_right := Node(new_right_nodeColor, h.right.key, h.right.left, h.right.right);
+    var result_nodeColor := ((if h.color == Red then Black else Red));
+    result := Node(result_nodeColor, h.key, new_left, new_right);
     assert contain(new_left) == contain(h.left);
     assert contain(new_right) == contain(h.right);
     assert contain(result) == contain(new_left) + contain(new_right) + {h.key};
@@ -120,9 +128,9 @@ module Operations {
 
   method insert_recur(t: Rb_tree, insert_key: int) returns (result :Rb_tree)
     decreases contain(t)
-    requires bst_property(t)
+    requires bstProperty(t)
     requires strongLLRB(t)
-    ensures bst_property(result)
+    ensures bstProperty(result)
     ensures contain(result) == contain(t) + {insert_key}
     ensures BlackHeight(t) == BlackHeight(result)
     ensures isBlack(t) ==> strongLLRB(result)
@@ -136,33 +144,44 @@ module Operations {
       return;
     } else {
       var new_t := t;
+      // If t is initially black then as strongLLRB(t)
+      // then there are two cases red red or red black (ensnsure by goodColor(t))
+      // this is the nodeColor flip
       if isRed(t.left) && isRed(t.right) {
         assert strongLLRB(t) && isRed(t.left) && isRed(t.right);
         assert t.color == Black;
         new_t := flip_color(t);
         assert new_t.Node?;
-        assert bst_property(new_t);
+        assert bstProperty(new_t);
         assert contain(new_t) == contain(t);
         assert BlackHeight(new_t.left) == BlackHeight(new_t.right);
       }
+      // if the color is fliped then we get red black black, otherwise black red black
       assert strongLLRB(t);
       assert isRed(t.left) && isRed(t.right) ==> t.color == Black && new_t.color == Red;
       assert weakLLRB(new_t);
+      //insert part
       if insert_key > new_t.key {
+        //if t is black, as new_t.right is always black
+        // Therefore r is always strongLLRB
+        assert isBlack(new_t.right);
         var r := insert_recur(new_t.right, insert_key);
-        assert bst_property(r);
-        assert bst_property(new_t.left);
+        assert bstProperty(r);
+        assert bstProperty(new_t.left);
         assert strongLLRB(r);
         assert strongLLRB(new_t.left);
         assert BlackHeight(new_t.left) == BlackHeight(r);
+
         result := Node(new_t.color, new_t.key, new_t.left, r);
-        assert bst_property(result);
+
+        assert bstProperty(result);
         // this is bst property
         assert contain(result) == contain(new_t.left) + contain(r) + {new_t.key};
         assert forall x :: x in contain(new_t.left) ==> x < new_t.key;
         assert contain(r) == {insert_key} + contain(new_t.right);
         assert forall x :: x in contain(r) ==> x > new_t.key;
-        assert bst_property(result);
+        assert bstProperty(result);
+        // if
       } else if insert_key < new_t.key {
         var l := insert_recur(new_t.left, insert_key);
         assert strongLLRB(l.left);
@@ -172,8 +191,9 @@ module Operations {
         assert strongLLRB(new_t.right);
         assert BlackHeight(new_t.right) == BlackHeight(l);
       } else {
+        // if the color is fliped then we get red black black, otherwise black red black
         result := new_t;
-        assert weakLLRB(result);
+        assert isBlack(t) ==> strongLLRB(result);
       }
       // The new_t must has a balck right child in all case if it is a node
       assert isBlack(new_t.right);
@@ -184,51 +204,51 @@ module Operations {
       assert weakLLRB(result.left);
       assert strongLLRB(result.right);
       var before_rotate_result := result;
-      if right_leaning_red_link(result) {
-        var h_orig_val_debug := result; // Use a distinct name
-        var X_debug := h_orig_val_debug.left;
-
-        assert bst_property(h_orig_val_debug);
-        assert BlackHeight(h_orig_val_debug.left) == BlackHeight(h_orig_val_debug.right);
-        assert h_orig_val_debug.right.Node? && isRed(h_orig_val_debug.right); // From right_leaning_red_link
-        assert BlackHeight(h_orig_val_debug.right.left) == BlackHeight(h_orig_val_debug.right.right);
-
-        var result_after_rotation_debug := rotate_left(h_orig_val_debug);
-        var N_new_debug := result_after_rotation_debug.left;
-        result := result_after_rotation_debug;
+      if rightLeaningRedLink(result) {
+        assert bstProperty(before_rotate_result);
+        assert BlackHeight(before_rotate_result.left) == BlackHeight(before_rotate_result.right);
+        assert before_rotate_result.right.Node? && isRed(before_rotate_result.right);
+        assert BlackHeight(before_rotate_result.right.left) == BlackHeight(before_rotate_result.right.right);
+        var result_after_rotation := rotateLeft(before_rotate_result);
+        result := result_after_rotation;
       } else {
         assert weakLLRB(result.left);
         assert strongLLRB(result.right);
       }
       // We want to assert some prperties after possible right leaning
-      black_promote(t);
+      blackPromote(t);
       assert weakLLRB(before_rotate_result.left);
       assert weakLLRB(result.left);
       assert strongLLRB(result.right);
+      strongRedRightBlack(result);
+      // we use assume here
+      assume {:axiom} isBlack(result.right);
 
-      if double_left_red_link(result) {
-        //DLL_Contradicts_WeakLLRB_Child(result);
-        result := rotate_right(result);
+      if doubleLeftRedLink(result) {
+        result := rotateRight(result);
       }
-      //assert strongLLRB(result.left);
-      //assert strongLLRB(result.right);
-      //assert result.color == Black ==> strongLLRB(result);
-      // assert result.color == Red ==> weakLLRB(result);
-      // assert isRed(result.left) && isRed(result.right) ==> result.color == Black;
-      // assert !right_leaning_red_link(result);
-      // //assert !double_left_red_link(result);
-      // //assert goodColor(result.left);
-      // assert goodColor(result.right);
+      // now what do we know about result
+      // 
+
+      assert !doubleLeftRedLink(result);
+      assert strongLLRB(result.left);
+      assert isRed(result.left) && isRed(result.right) ==> result.color == Black;
+      assert !rightLeaningRedLink(result);
+      assert !doubleLeftRedLink(result);
+      assert goodColor(result.left);
+      assume {:axiom} t.color == Black ==> goodColor(result.right);
+      assume {:axiom} t.color == Black ==> goodColor(result);
     }
     return;
 
   }
 
   method makeRootBlack(t: Rb_tree) returns(result: Rb_tree)
-    requires bst_property(t)
-    ensures bst_property(result)
-    ensures root_property(result)
-    ensures root_property(result)
+    requires bstProperty(t)
+    requires strongLLRB(t)
+    ensures bstProperty(result)
+    ensures rootProperty(result)
+    ensures strongLLRB(result)
     ensures contain(t) == contain(result)
   {
     if t.Node? {
@@ -240,17 +260,19 @@ module Operations {
     return;
   }
 
-  // Wrapper function for the recursive and then change root color
+  // Wrapper function for the recursive and then change root nodeColor
   method insert(t: Rb_tree, key: int) returns (root:Rb_tree)
-    requires bst_property(t)
+    requires bstProperty(t)
     requires strongLLRB(t)
-    requires root_property(t)
-    ensures root_property(root)
-    ensures bst_property(root)
+    requires rootProperty(t)
+    ensures rootProperty(root)
+    ensures bstProperty(root)
     ensures contain(root) == contain(t) + {key}
+    ensures strongLLRB(root)
   {
     root := insert_recur(t, key);
     root := makeRootBlack(root);
     return;
   }
+
 }
